Weidenbach_Book/IsaSAT/IsaSAT_Simplify_Forward_Subsumption_LLVM.thy
@@ -814,13 +814,27 @@ lemma isa_forward_subsumption_all_wl_invI:
   apply normalize_goal+
   by (auto simp: isasat_fast_relaxed_def)
 
-sepref_register empty_occs2_st forward_subsumption_finalize
+sepref_register empty_occs2_st forward_subsumption_finalize schedule_next_subsume_st
 
 sepref_def mark_added_clause_heur2_impl
   is \<open>uncurry mark_added_clause_heur2\<close>
   :: \<open>isasat_bounded_assn\<^sup>d *\<^sub>a sint64_nat_assn\<^sup>k \<rightarrow>\<^sub>a isasat_bounded_assn\<close>
   unfolding mark_added_clause_heur2_def
   apply (annot_snat_const \<open>TYPE(64)\<close>)
+  by sepref
+
+lemma schedule_next_subsume_st_alt_def:
+  \<open>schedule_next_subsume_st b S = (let (heur, S) = extract_heur_wl_heur S;
+      heur = schedule_next_subsume b  heur in
+      update_heur_wl_heur heur S)\<close>
+  by (auto simp: schedule_next_subsume_st_def Let_def state_extractors
+    split: isasat_int_splits)
+
+sepref_def schedule_next_subsume_st
+  is \<open>uncurry (RETURN oo schedule_next_subsume_st)\<close>
+  :: \<open>word64_assn\<^sup>k *\<^sub>a isasat_bounded_assn\<^sup>d \<rightarrow>\<^sub>a isasat_bounded_assn\<close>
+  supply [[goals_limit=1]]
+  unfolding schedule_next_subsume_st_alt_def
   by sepref
 
 sepref_def forward_subsumption_finalize
@@ -843,11 +857,31 @@ sepref_def isa_forward_subsumption_all_impl
   apply (annot_snat_const \<open>TYPE(64)\<close>)
   by sepref
 
-(*TODO this should become a should_forward_subsume with different scheduling than pure literals*)
-sepref_def should_inprocess_st
-  is \<open>RETURN o should_inprocess_st\<close>
+
+lemma get_subsumption_opts_alt_def:
+  \<open>get_subsumption_opts S = (case S of IsaSAT M N D i W ivmtf icount ccach lbd outl stats heur aivdom clss opts arena occs \<Rightarrow> opts_subsumption opts)\<close>
+  by (cases S) (auto simp: get_subsumption_opts_def)
+
+sepref_def get_subsumption_opts_impl
+  is \<open>RETURN o get_subsumption_opts\<close>
   :: \<open>isasat_bounded_assn\<^sup>k \<rightarrow>\<^sub>a bool1_assn\<close>
-  unfolding should_inprocess_st_def
+  unfolding get_subsumption_opts_alt_def
+  by sepref
+
+lemma next_subsume_schedule_st_def:
+  \<open>next_subsume_schedule_st S = (case S of IsaSAT M N D i W ivmtf icount ccach lbd outl stats heur aivdom clss opts arena occs \<Rightarrow> next_subsume_schedule heur)\<close>
+  by (cases S) (auto simp: next_subsume_schedule_st_def)
+
+sepref_def next_subsume_schedule_st_impl
+  is \<open>RETURN o next_subsume_schedule_st\<close>
+  :: \<open>isasat_bounded_assn\<^sup>k \<rightarrow>\<^sub>a word_assn\<close>
+  unfolding next_subsume_schedule_st_def
+  by sepref
+
+sepref_def should_subsume_st
+  is \<open>RETURN o should_subsume_st\<close>
+  :: \<open>isasat_bounded_assn\<^sup>k \<rightarrow>\<^sub>a bool1_assn\<close>
+  unfolding should_subsume_st_def
   by sepref
 
 sepref_def isa_forward_subsume_impl
